post-cip/formal-crypto/lean/src/Leioscrypto/Certificate.lean
@@ -7,14 +7,21 @@ import Leioscrypto.Types
 namespace Leioscrypto
 
 
-structure Certificate (e : ElectionContext) where
+structure Certificate where
   electionId : ElectionId
   ebHash : BlockHash
   persistentVotes : List PoolIndex
   nonpersistentVotes : List (PoolIndex × BLS.Signature)
   sigma_tilde_eid : Option BLS.Signature
   sigma_tilde_m : BLS.Signature
-deriving Repr
+
+namespace Certificate
+
+  structure WellFormed (c : Certificate) : Prop where
+    wf_sigma_tilde_eid : c.sigma_tilde_eid.elim True BLS.Signature.WellFormed
+    wf_sigma_tilde_m : c.sigma_tilde_m.WellFormed
+
+end Certificate
 
 
 end Leioscrypto
