post-cip/formal-crypto/lean/src/Leioscrypto/Types.lean
@@ -7,31 +7,27 @@ def Slot := Nat
 
 
 def Coin := Rat
-  deriving Repr, OfNat, LT, LE
+  deriving OfNat, LT, LE
 
 
 def PraosNonce := BitVec 256
-  deriving Repr
 
 
 def BlockHash := BitVec 256
-  deriving Repr
 
 
 def PoolKeyHash := BitVec 224
-  deriving Repr, BEq, LawfulBEq
+  deriving BEq, LawfulBEq
 
 
 def ColdKeySignature := BitVec 256
-  deriving Repr, BEq
+  deriving BEq
 
 
 def PoolIndex := Nat
-  deriving Repr
 
 
 def ElectionId := Nat
-  deriving Repr
 
 
 end Leioscrypto
